Refactors
- Pack own_admin in a bupd.
- Better SLRed

Note: lacking proper adequacy, so this doesn't mean that much.

theories/iris_system/invariants.v
@@ -30,7 +30,7 @@ Section invariants.
 
   Global Instance subG_invG : subG invΣ Σ → subG invΓ Γ → invG.
   Proof using. solve_inG. Defined.
-  
+
   (* Initial resources for invariants *)
   Definition ir_ownIRA : DRA_mk ownIRA := λ n, allocs_auth _ (λ i, True).
   Lemma ir_ownIRA_valid : ✓ ir_ownIRA.
@@ -46,6 +46,9 @@ End invariants.
 Global Arguments invG : clear implicits.
 Hint Unfold invG_I invG_E subG_invG subG_inG : GRA_index.
 
+Axiom invariant_name : gname.
+Axiom enabled_name : gname.
+
 Section predicates.
   Context `{!subG (Γ : HRA) Σ, !invG Γ Σ α}.
   Local Existing Instances invG_I invG_E.
@@ -55,7 +58,7 @@ Section predicates.
   Definition ownIR {n} i (p : GTerm.t n) : ownIRA :=
     discrete_fun_singleton n (allocs_frag i (None, (to_agree p))).
   Definition ownI {n} i (p : GTerm.t n) : iProp Σ :=
-    own base_γ (ownIR i p).
+    own invariant_name (ownIR i p).
 
   Global Instance ownI_persistent n i p : Persistent (@ownI n i p).
   Proof using. apply _. Qed.
@@ -64,16 +67,16 @@ Section predicates.
   Definition ownI_reserveR n (X : coPset) : ownIRA :=
     discrete_fun_singleton n (allocs_auth _ (λ i, i ∈ X)).
   Definition ownI_reserve n (X : coPset) : iProp Σ :=
-    own base_γ (ownI_reserveR n X).
-  Definition ownD {n} i p : iProp Σ :=
-    own base_γ (discrete_fun_singleton n (allocs_frag i (Some (Excl ()), to_agree p))).
+    own invariant_name (ownI_reserveR n X).
+  Definition ownD {n} i (p : GTerm.t n) : iProp Σ :=
+    own invariant_name (discrete_fun_singleton n (allocs_frag i (Some (Excl ()), to_agree p))).
 
   (* authorative resource for wsats *)
   Definition wsat_authR (b : nat) (X : coPset) : ownIRA :=
     (λ n, if (decide (n < b)) then ε else (allocs_auth _ (λ i, i ∈ X))).
-  Definition wsat_auth b X : iProp Σ := own base_γ (wsat_authR b X).
+  Definition wsat_auth b X : iProp Σ := own invariant_name (wsat_authR b X).
 
-  Definition ownE (E : coPset) : iProp Σ := own base_γ (CoPset E).
+  Definition ownE (E : coPset) : iProp Σ := own enabled_name (CoPset E).
 
   (* predicate rules *)
   Lemma ownE_exploit (E1 E2 : coPset) : ownE E1 ∗ ownE E2 ⊢ ⌜E1 ## E2⌝.
@@ -143,7 +146,8 @@ Section predicates.
 End predicates.
 
 Section wsat.
-  Context `{@GATIntp.t (domain Σ) α, !invG Γ Σ α, !subG Γ Σ}.
+  Context `{Σ : GRA, Γ : HRA}.
+  Context `{@GATIntp.t (iPropI Σ) α, !invG Γ Σ α, !subG Γ Σ}.
 
   Definition inv_satall {n} (I : gmap positive (GTerm.t n)) : iProp Σ :=
     [∗ map] i ↦ p ∈ I, ownI i p ∗ ((⟦p⟧ ∗ ownD i p) ∨ ownE {[i]}).
@@ -154,23 +158,20 @@ Section wsat.
       let dom := gset_to_coPset (dom I) in
       ⌜dom ⊆ X⌝ ∗ inv_satall I ∗ ownI_reserve n (X ∖ dom).
 
-  Lemma gset_to_coPset_union X Y : gset_to_coPset (X ∪ Y) = gset_to_coPset X ∪ gset_to_coPset Y.
-  Proof using.
-    unfold_leibniz; split.
-    { intros ?%elem_of_gset_to_coPset%elem_of_union; rewrite elem_of_union; des; [left | right];
-        apply elem_of_gset_to_coPset; done.
-    }
-    { intros [Hin|Hin]%elem_of_union; apply elem_of_gset_to_coPset in Hin;
-        apply elem_of_gset_to_coPset, elem_of_union; eauto.
-    }
-  Qed.
+  Local Ltac simplify_gset_to_coPset :=
+    set_unfold; setoid_rewrite elem_of_gset_to_coPset; set_unfold.
+
+  Lemma gset_to_coPset_union X Y :
+    gset_to_coPset (X ∪ Y) = gset_to_coPset X ∪ gset_to_coPset Y.
+  Proof using. by simplify_gset_to_coPset. Qed.
 
   Lemma gset_to_coPset_empty : gset_to_coPset ∅ = ∅.
-  Proof using. unfold_leibniz; ii; ss. Qed.
+  Proof using. set_solver. Qed.
 
   Lemma gset_to_coPset_singleton i : gset_to_coPset {[i]} = {[i]}.
   Proof using.
-    unfold_leibniz; split; rewrite elem_of_gset_to_coPset ?elem_of_singleton //.
+    (* FIXME: set_unfold unfolds way too much *)
+    apply leibniz_equiv => ?. rewrite elem_of_gset_to_coPset. set_solver.
   Qed.
 
   Lemma inv_satall_split {n} (X Y : gmap positive (GTerm.t n)) :
@@ -329,7 +330,8 @@ Section wsat.
 End wsat.
 
 Section wsats.
-  Context `{@GATIntp.t (domain Σ) α, !invG Γ Σ α, !subG Γ Σ}.  
+  Context `{Σ : GRA, Γ : HRA}.
+  Context `{@GATIntp.t (iPropI Σ) α, !invG Γ Σ α, !subG Γ Σ}.
   Local Existing Instances invG_I invG_E.
 
   Lemma wsat_authR_valid n X : ✓ (wsat_authR n X).
@@ -360,6 +362,10 @@ Section wsats.
   Qed.
 
   Definition wsatl n X : iProp Σ := [∗ list] x ∈ (seq 0 n), wsat x X.
+
+  Lemma wsatl_S n X :
+    wsatl (S n) X ⊣⊢ wsatl n X ∗ wsat n X.
+  Proof. rewrite /wsatl seq_S left_id_L big_sepL_snoc //. Qed.
 
   Lemma wsatl_acc n m X : n < m → wsatl m X ⊣⊢ wsat n X ∗ (wsat n X -∗ wsatl m X).
   Proof using.
@@ -429,14 +435,14 @@ Section wsats.
   Qed.
 
   (* For cancellation *)
-  Lemma make_wsats : own base_γ (ir_ownIRA) ∗ own base_γ ir_ownERA ⊢ wsats 0 ⊤ ∗ ownE ⊤.
+  Lemma make_wsats : own invariant_name (ir_ownIRA) ∗ own enabled_name ir_ownERA ⊢ wsats 0 ⊤ ∗ ownE ⊤.
   Proof.
     rewrite /ir_ownIRA /wsats; iIntros "[I E]"; iSplitL "I"; ss. rewrite /wsatl //=. iFrame.
   Qed.
 
   (* Definitions for fancy updates & invariants *)
   Local Definition uPred_fupd_def b (E E1 E2 : coPset) (P : iProp Σ) : iProp Σ :=
-    wsatl b E ∗ ownE E1 ∗ own_admin ==∗ (wsatl b E ∗ ownE E2 ∗ own_admin ∗ P).
+    wsatl b E ∗ ownE E1 o==∗ (wsatl b E ∗ ownE E2 ∗ P).
   Local Definition uPred_fupd_aux : seal (@uPred_fupd_def). Proof using. by eexists. Qed.
   Definition uPred_fupd := uPred_fupd_aux.(unseal).
   Local Definition uPred_fupd_eq : @uPred_fupd = @uPred_fupd_def := uPred_fupd_aux.(seal_eq).
@@ -446,31 +452,36 @@ Section wsats.
   Lemma uPred_fupd_mixin n E : BiFUpdMixin (iProp Σ) (uPred_fupd n E).
   Proof using.
     split.
-    - rewrite /updates.fupd uPred_fupd_eq. solve_proper.
+    - rewrite uPred_fupd_unseal. solve_proper.
     - intros E1 E2 (E1''&->&?)%subseteq_disjoint_union_L.
-      rewrite /fupd uPred_fupd_eq /uPred_fupd_def ownE_op //.
-      iIntros "[$ [[$ $] $]] !> [$ [$ $]] //".
-    - rewrite /fupd uPred_fupd_eq /uPred_fupd_def /wsats /bi_except_0.
-      iIntros (E1 E2 P) "[H | H]"; iFrame.
-      iDestruct (uPred.later_eq with "H") as "H"; by iFrame.
-    - rewrite /fupd uPred_fupd_eq /uPred_fupd_def /wsats.
+      rewrite uPred_fupd_unseal /uPred_fupd_def ownE_op //.
+      iIntros "[$ [$ $]] !> [$ $] //".
+    - rewrite uPred_fupd_unseal.
+      iIntros (E1 E2 P) ">H [Hw HE]". iApply "H"; by iFrame.
+    - rewrite uPred_fupd_unseal /uPred_fupd_def /wsats.
       iIntros (E1 E2 P Q HPQ) "HP HwE". rewrite -HPQ. by iApply "HP".
-    - rewrite /fupd uPred_fupd_eq /uPred_fupd_def /wsats. iIntros (E1 E2 E3 P) "HP HwE".
-      iMod ("HP" with "HwE") as "[? [? [? HP]]]". iApply "HP"; by iFrame.
+    - rewrite uPred_fupd_unseal /uPred_fupd_def /wsats. iIntros (E1 E2 E3 P) "HP HwE".
+      iMod ("HP" with "HwE") as "[? [? HP]]". iApply "HP"; by iFrame.
     - intros E1 E2 Ef P HE1Ef.
-      rewrite /fupd uPred_fupd_eq /uPred_fupd_def ownE_op //.
-      iIntros "Hupd [W [[E Ef] O]]".
+      rewrite uPred_fupd_unseal /uPred_fupd_def ownE_op //.
+      iIntros "Hupd [W [E Ef]]".
       (* iPoseProof (wsatl_split with "W") as "[W1 Wf]"; ss. *)
-      iMod ("Hupd" with "[W E O]") as "[W [E2 [$ P]]]"; iFrame.
+      iMod ("Hupd" with "[W E]") as "[W [E2 P]]"; iFrame.
       iPoseProof (ownE_exploit with "[Ef E2]") as "%DISJ"; first iFrame.
       rewrite ownE_op //; iFrame; by iApply "P".
-    - rewrite /fupd uPred_fupd_eq /uPred_fupd_def /wsats. by iIntros (????) "[HwP $]".
+    - rewrite uPred_fupd_unseal /uPred_fupd_def /wsats. by iIntros (????) "[HwP $]".
   Qed.
-  Global Instance uPred_bi_fupd n E : BiFUpd (iProp Σ) :=
+  Global Instance uPred_bi_fupd n E : BiFUpd (iPropI Σ) :=
     {| bi_fupd_mixin := (uPred_fupd_mixin n E) |}.
   Global Instance uPred_bi_bupd_fupd n E :
-    @BiBUpdFUpd (iProp Σ) (uPred_bi_bupd Σ) (uPred_bi_fupd n E).
-  Proof using. rewrite /BiBUpdFUpd uPred_fupd_unseal. by iIntros (??) ">? [$ [$ $]] !>". Qed.
+    @BiBUpdFUpd (iPropI Σ) _ (uPred_bi_fupd n E).
+  Proof using. rewrite /BiBUpdFUpd uPred_fupd_unseal. by iIntros (??) ">? [$ $] !>". Qed.
+  Global Instance uPred_bi_own_bupd_fupd n Ew :
+    @BiBUpdFUpd (iPropI Σ) uPred_bi_bupd_own (uPred_bi_fupd n Ew).
+  Proof using.
+    rewrite /BiBUpdFUpd uPred_fupd_unseal.
+    iIntros (E P) "HUpd ($ & $)". by iApply "HUpd".
+  Qed.
 
   (* definition of an invariant *)
   Local Definition inv_def {n : level} (N : namespace) (p : GTerm.t n) : iProp Σ :=
@@ -482,6 +493,7 @@ Section wsats.
   Global Instance inv_persistent n N p : Persistent (inv n N p).
   Proof using. rewrite inv_eq /inv_def. apply _. Qed.
 
+  (* TODO: Move *)
   (** Turns a pure proposition into a resource **)
   Definition pure_res (P : Prop) : Σ :=
     if excluded_middle_informative P
@@ -498,13 +510,13 @@ Section wsats.
 
     split; i; eapply Own_general_completeness in H1; exfalso; cycle 1.
     { eapply n, Own_pure_soundness; et. }
-  
+
     eapply Own_wand_valid in H0; cycle 1.
     { iIntros "X". iApply H1. et. }
-    assert (F := own.iRes_singleton_validI base_γ (CoPset ⊤ ⋅ CoPset ⊤)).
-    assert (Own ε ⊢ ✓ (CoPset ⊤ ⋅ CoPset ⊤ ))%I.
-    { iIntros "_". iApply F. et. }
-    exploit (uPred_primitive.ownM_general_soundness ε (✓ (CoPset ⊤ ⋅ CoPset ⊤))); eauto using ucmra_unit_valid.
+    assert (F := own.iRes_singleton_valid base_γ (CoPset ⊤ ⋅ CoPset ⊤)).
+    assert (Own ε ⊢ ⌜✓ (CoPset ⊤ ⋅ CoPset ⊤ )⌝)%I.
+    { iIntros "_". iPureIntro. apply F. et. }
+    exploit (uPred_primitive.ownM_general_soundness ε (⌜✓ (CoPset ⊤ ⋅ CoPset ⊤)⌝)); eauto using ucmra_unit_valid.
     { rr in H2. rewrite own.Own_eq /own.Own_def in H2. et. }
     intro V. rr in V. revert V. rewrite seal_eq. ss.
   Qed.
@@ -518,8 +530,9 @@ Section wsats.
 End wsats.
 
 Notation fupd_ex n E :=
-  (@fupd (bi_car (iProp _)) (@bi_fupd_fupd _ (uPred_bi_fupd n E))) (only parsing).
+  (@fupd (bi_car _) (@bi_fupd_fupd _ (uPred_bi_fupd n E))) (only parsing).
 
+(* TODO: better notation formatting *)
 Notation "'=|' n ',' E '|={' E1 ',' E2 '}=>' P" := (fupd_ex n E E1 E2 P) (at level 90) : stdpp_scope.
 Notation "P '=|' n ',' E '|={' E1 ',' E2 '}=∗' Q" := (P -∗ =|n, E|={E1,E2}=> Q) (at level 90) : stdpp_scope.
 
@@ -533,12 +546,13 @@ Notation "'=|' n ',' E '|={' E1 '}=>' P" := (=|n, E|={E1, E1}=> P)%I (at level 9
 Notation "P '=|' n ',' E '|={' E1 '}=∗' Q" := (P -∗ =|n, E|={E1}=> Q)%I (at level 90) : bi_scope.
 
 Section fancy_updates.
-  Context `{@GATIntp.t (domain Σ) α, !invG Γ Σ α, !subG Γ Σ}.  
+  Context `{Σ : GRA, Γ : HRA}.
+  Context `{@GATIntp.t (iProp Σ) α, !invG Γ Σ α, !subG Γ Σ}.
   Implicit Types n m : level.
   Implicit Types N : namespace.
   Implicit Types E : coPset.
 
-  Lemma fupd_mon n m E E1 E2 P : n <= m → =|n, E|={E1, E2}=> P -∗ =|m, E|={E1, E2}=> P.
+  Lemma fupd_mon n m E E1 E2 P : n <= m → =|n, E|={E1, E2}=> P ⊢ =|m, E|={E1, E2}=> P.
   Proof using.
     intros LT; rewrite ?uPred_fupd_unseal /uPred_fupd_def /wsats.
     iIntros "P [W E]".
@@ -550,7 +564,7 @@ Section fancy_updates.
 
   Lemma fupd_mon_namespace n Ew Ew' E1 E2 P :
     Ew' ⊆ Ew →
-    =|n, Ew'|={E1, E2}=> P -∗ =|n, Ew|={E1, E2}=> P.
+    =|n, Ew'|={E1, E2}=> P ⊢ =|n, Ew|={E1, E2}=> P.
   Proof using.
     iIntros (?) "P"; rewrite ?uPred_fupd_unseal /uPred_fupd_def; iIntros "[W E]".
     rewrite {1}(union_difference_L Ew' Ew) // wsatl_split; last set_solver.
@@ -560,20 +574,15 @@ Section fancy_updates.
 End fancy_updates.
 
 Section inv.
-  Context `{@GATIntp.t (domain Σ) α, !invG Γ Σ α, !subG Γ Σ}.  
+  Context `{Σ : GRA, Γ : HRA}.
+  Context `{@GATIntp.t (iProp Σ) α, !invG Γ Σ α, !subG Γ Σ}.
   Implicit Types (n : level) (N : namespace) (E : coPset).
-
-  Lemma own_alloc `{!inG A Σ} (a : A) Ew E : ✓ a → ⊢ =|0, Ew|={E}=> ∃ γ, own γ a.
-  Proof.
-    iIntros (?); rewrite uPred_fupd_unseal /uPred_fupd_def; iIntros "[$ [$ O]]".
-    by iApply own_admin_alloc.
-  Qed.
 
   Lemma inv_alloc {n} (p : GTerm.t n) m E Ew N :
     n < m → ↑N ⊆ Ew → ⟦p⟧ =|m, Ew|={E}=∗ inv n N p.
   Proof using.
     rewrite ?uPred_fupd_unseal /uPred_fupd_def ?inv_eq /inv_def.
-    iIntros (LT Hsub) "P [W [E $]]".
+    iIntros (LT Hsub) "P [W E]".
     iPoseProof (wsatl_acc n with "W") as "[W A]"; first done.
     iMod (wsat_ownI_alloc Ew (↑N) p with "[W P]") as "[[%i [%Hi #HiP]] W]"; ss.
     { apply coPset_infinite_finite, nclose_infinite. }
@@ -589,36 +598,37 @@ Section inv.
     rewrite ?uPred_fupd_unseal /uPred_fupd_def ?inv_eq /inv_def.
     iDestruct 1 as (i) "[Hi #HiP]".
     iDestruct "Hi" as % ?%elem_of_subseteq_singleton.
-    rewrite {1}(wsatl_acc n) //; iIntros "[[W ACC] [E O]]".
+    rewrite {1}(wsatl_acc n) //; iIntros "[[W ACC] E]".
     rewrite {1}(union_difference_L (↑ N) E) // ownE_op; last set_solver.
     rewrite {1}(union_difference_L {[ i ]} (↑ N)) // ownE_op; last set_solver.
     iDestruct "E" as "[[E1 E3] E2]".
     iPoseProof (wsat_ownI_open with "[HiP W E1]") as "[P [W D2]]"; try by iFrame.
     { set_solver. }
     iPoseProof ("ACC" with "W") as "W"; iFrame.
-    rewrite {1}(wsatl_acc n) //; iIntros "!> P [[W R] [E $]]".
+    rewrite {1}(wsatl_acc n) //; iIntros "!> P [[W R] E]".
     iPoseProof (wsat_ownI_close with "[W P D2]") as "[W E']"; try by iFrame. { set_solver. }
     rewrite {2}(union_difference_L (↑ N) E) // ownE_op; last set_solver.
     rewrite {3}(union_difference_L {[ i ]} (↑ N)) // ownE_op; last set_solver; iFrame.
     iModIntro; iApply "R"; iFrame.
   Qed.
 
-  Global Instance from_modal_fupd n Ew E1 E2 P :
+  (* Global Instance from_modal_fupd n Ew E1 E2 P :
     FromModal (E2 ⊆ E1) modality_id (=|n, Ew|={E1,E2}=> P) (=|n, Ew|={E1,E2}=> P) P | 1.
   Proof using.
     rewrite /FromModal ?uPred_fupd_unseal /uPred_fupd_def ?inv_eq /inv_def /=.
     iIntros (IN) "$ W !>".
     rewrite (union_difference_L E2 E1) // /wsats ownE_op; last set_solver.
     iDestruct "W" as "[$ [[$ _] $]]".
-  Qed.
+  Qed. *)
 
-  Global Instance into_acc_inv n m Ew E N p :
+  Global Instance into_acc_inv n m Ew E N p P:
+    SLRed n p P →
     IntoAcc (inv n N p) (n < m ∧ ↑N ⊆ E ∧ E ⊆ Ew) True
             (fupd_ex m Ew E (E ∖ ↑N))
             (fupd_ex m Ew (E ∖ ↑N) E)
-            (λ _ : (), ⟦p⟧) (λ _ : (), ⟦p⟧) (λ _ : (), None).
+            (λ _ : (), P) (λ _ : (), P) (λ _ : (), None).
   Proof using.
-    rewrite /IntoAcc /accessor bi.exist_unit.
+    rewrite /IntoAcc /accessor bi.exist_unit => HpP. rewrite <-HpP.
     iIntros ((? & ?)) "#INV _". by iApply inv_acc; set_solver.
   Qed.
 
@@ -631,29 +641,21 @@ Section inv.
     iIntros ([LE [SUB SUB2]]) "[P K]".
     iPoseProof (fupd_mon n m with "P") as "P"; ss.
     iPoseProof (fupd_mon_namespace _ Ew with "P") as "P"; ss.
-    rewrite ?uPred_fupd_unseal /uPred_fupd_def ?inv_eq /inv_def /=.
-    iIntros "[WL [E O]]".
-    rewrite {2}(union_difference_L E0 E2) // (ownE_op (E0)); last set_solver.
-    iDestruct "E" as "[E1 E2]".
-    iPoseProof ("P" with "[WL E1 O]") as "> [W [E [O P]]]"; first iFrame.
-    iApply ("K" with "P [W E E2 O]"); iFrame.
-    iPoseProof (ownE_exploit with "[E E2]") as "%D"; iFrame.
-    rewrite ownE_op; ss; iFrame.
+    iApply fupd_mask_frame; [exact SUB|].
+    iMod "P". iApply ("K" with "P").
   Qed.
 
   Global Instance elim_modal_fupd_fupd_simple p n m Ew E1 E2 E3 P Q :
     ElimModal (n <= m) p false
               (=|n, Ew|={E1,E2}=> P) P (=|m, Ew|={E1,E3}=> Q) (=|m, Ew|={E2,E3}=> Q).
   Proof using.
-    rewrite /ElimModal bi.intuitionistically_if_elim.
-    iIntros (LE) "[P K]".
-    iPoseProof (fupd_mon n m with "P") as "P"; ss.
-    iMod "P". iMod ("K" with "P") as "K"; iModIntro; ss.
+    intros ?. rewrite (fupd_mon n m) //. by apply: elim_modal.
   Qed.
 End inv.
 
 Section winv.
-  Context `{@GATIntp.t (domain Σ) α, !invG Γ Σ α, !subG Γ Σ}.  
+  Context `{Σ : GRA, Γ : HRA}.
+  Context `{@GATIntp.t (iProp Σ) α, !invG Γ Σ α, !subG Γ Σ}.
 
   Definition winv (Ep : coPset * coPset) : iProp Σ :=
     match Ep with
@@ -700,21 +702,22 @@ Section winv.
   Lemma winv_fupd n Ew E1 E2 P :
     =|n, Ew|={E1, E2}=> P ⊢ winv (Ew, E1) ==∗ winv (Ew, E2) ∗ P.
   Proof.
-    rewrite uPred_fupd_unseal /uPred_fupd_def; iIntros "F [O [E [%n' W]]]".
+    rewrite uPred_fupd_unseal /uPred_fupd_def own_bupd_unseal /own_bupd;
+    iIntros "F [O [E [%n' W]]]".
     destruct (decide (n < n')).
     { iDestruct "W" as "[A L]".
       replace n' with (n + (n' - n)) at 2 by lia.
       rewrite {3}/wsatl seq_app /=.
       iPoseProof (big_sepL_app with "L") as "[W R]"; eauto.
-      iMod ("F" with "[W E O]") as "[W [E [O P]]]"; first iFrame.
+      iMod ("F" with "[$W $E] O") as "[O [W [E P]]]".
       iCombine "W" "R" as "W"; rewrite -big_sepL_app -seq_app /=.
       iFrame. replace (n + (n' - n)) with n' by lia; done.
     }
     { iPoseProof (wsats_mon n' n with "W") as "> [W L]"; first lia.
-      iMod ("F" with "[L E O]") as "[$ [$ [$ $]]]"; iFrame; done.
+      iMod ("F" with "[L E] O") as "($&$&$&$)"; iFrame; done.
     }
   Qed.
-  (* TODO : move to invariants.v *)
+
   Global Instance elim_winv_simple Ew Ew' E0 E1 n P Q p :
     ElimModal
       (Ew' ⊆ Ew) p false
@@ -746,7 +749,7 @@ Ltac unfold_left :=
   | |- context [InitRes.R (discrete_fun_singleton _ _)] => rewrite ?InitRes.R_index
   end.
 
-Ltac solve_index H := 
+Ltac solve_index H :=
   eapply eq_ind; first iExact H;
   unfold_own;
   etrans;
@@ -829,12 +832,12 @@ Ltac _simplify_res :=
       end
   end.
 
-Ltac _wsats_res := 
+Ltac _wsats_res :=
   lazymatch goal with
   |- context[environments.Esnoc _ (INamed ?I) (own base_γ (ir_ownIRA))] =>
-  lazymatch goal with 
+  lazymatch goal with
   |- context[environments.Esnoc _ (INamed ?E) (own base_γ (ir_ownERA))] =>
-    let Pat := fresh "Pat" in      
+    let Pat := fresh "Pat" in
     pose (Pat := ("[" ++ I ++ " " ++ E  ++ "]")%string);
     compute in Pat;
     iPoseProof (make_wsats with Pat) as "[U W]"; [by iFrame|];
