theories/simulations/msim/ISim.v
@@ -121,7 +121,7 @@ Section SIM.
 
   Global Instance isim_elim_upd r g {Rs Rt} RR ps pt sti_src sti_tgt P p :
     ElimModal True p false ( |==> P)%I P
-      (@isim r g Rs Rt RR ps pt sti_src sti_tgt) 
+      (@isim r g Rs Rt RR ps pt sti_src sti_tgt)
       (isim r g RR ps pt sti_src sti_tgt).
   Proof using.
     unfold ElimModal. rewrite bi.intuitionistically_if_elim.
@@ -220,7 +220,7 @@ Section SIM.
   Lemma isim_tau_tgt r g ps pt {Rs Rt} RR st_src st_tgt i_src i_tgt :
     @isim r g Rs Rt RR ps true (st_src, i_src) (st_tgt, i_tgt)
     ⊢ @isim r g Rs Rt RR ps pt (st_src, i_src) (st_tgt, tau;; i_tgt).
-  Proof using. 
+  Proof using.
     by split; intros x wfx sim; guclo msimC_spec; econs; esplits; eauto; econs; eauto.
   Qed.
 
@@ -255,7 +255,7 @@ Section SIM.
     guclo msimC_spec; econs; esplits; eauto; econs; eauto; i.
     eapply isim_init; eauto.
   Qed.
-  
+
   Lemma isim_choose_src X r g ps pt {Rs Rt} RR st_src st_tgt k_src i_tgt :
     (∃ x, @isim r g Rs Rt RR true pt (st_src, k_src x) (st_tgt, i_tgt))
     ⊢ @isim r g Rs Rt RR ps pt (st_src, trigger (Choose X) >>= k_src) (st_tgt, i_tgt).
@@ -270,7 +270,7 @@ Section SIM.
   Lemma isim_choose_tgt X r g ps pt {Rs Rt} RR st_src st_tgt i_src k_tgt :
     (∀ x, @isim r g Rs Rt RR ps true (st_src, i_src) (st_tgt, k_tgt x))
     ⊢ @isim r g Rs Rt RR ps pt (st_src, i_src) (st_tgt, trigger (Choose X) >>= k_tgt).
-  Proof using. 
+  Proof using.
     split; intros x wfx SIM; guclo msimC_spec; econs; esplits; eauto; econs; eauto; i.
     eapply Own_general_completeness in SIM; eauto.
     eapply isim_init; eauto.
@@ -284,7 +284,7 @@ Section SIM.
     i. iIntros "H". unfold assume. rewrite bind_bind.
     iApply isim_take_src. rewrite bind_ret_l. eauto.
   Qed.
-  
+
   Lemma isim_asm_tgt (P : Prop) r g ps pt {Rs Rt} RR st_src st_tgt i_src k_tgt :
     P →
     @isim r g Rs Rt RR ps true (st_src, i_src) (st_tgt, k_tgt ())
@@ -294,7 +294,7 @@ Section SIM.
     iApply isim_take_tgt. rewrite bind_ret_l. eauto.
     Unshelve. eauto.
   Qed.
-  
+
   Lemma isim_guar_src (P : Prop) r g ps pt {Rs Rt} RR st_src st_tgt k_src i_tgt :
     ⌜P⌝ ∗ @isim r g Rs Rt RR true pt (st_src, k_src ()) (st_tgt, i_tgt)
     ⊢ @isim r g Rs Rt RR ps pt (st_src, guarantee P >>= k_src) (st_tgt, i_tgt).
@@ -307,7 +307,7 @@ Section SIM.
   Lemma isim_guar_tgt (P : Prop) r g ps pt {Rs Rt} RR st_src st_tgt i_src k_tgt :
     (∀ (_:P), @isim r g Rs Rt RR ps true (st_src, i_src) (st_tgt, k_tgt ()))
     ⊢ @isim r g Rs Rt RR ps pt (st_src, i_src) (st_tgt, guarantee P >>= k_tgt).
-  Proof using. 
+  Proof using.
     i. iIntros "H". unfold guarantee. rewrite bind_bind.
     iApply isim_choose_tgt. rewrite bind_ret_l. eauto.
   Qed.
@@ -333,7 +333,7 @@ Section SIM.
       + esplits; try eassumption. apply String.eqb_refl.
       + i. rewrite Heq in H2. ss.
   Qed.
-  
+
   Lemma isim_sput_tgt r g ps pt {Rs Rt} RR k v st_src st_tgt i_src k_tgt :
     @isim r g Rs Rt RR ps true (st_src, i_src) (alist_upd k v st_tgt, k_tgt tt)
     ⊢ @isim r g Rs Rt RR ps pt (st_src, i_src) (st_tgt, trigger (SPut k v) >>= k_tgt).
@@ -355,7 +355,7 @@ Section SIM.
       + esplits; try eassumption. apply String.eqb_refl.
       + i. rewrite Heq in H2. ss.
   Qed.
-  
+
   Lemma isim_sget_src r g ps pt {Rs Rt} RR k st_src st_tgt k_src i_tgt :
     @isim r g Rs Rt RR true pt (st_src, k_src (or_else (alist_find k st_src) tt↑)) (st_tgt, i_tgt)
     ⊢ @isim r g Rs Rt RR ps pt (st_src, trigger (SGet k) >>= k_src) (st_tgt, i_tgt).
@@ -377,7 +377,7 @@ Section SIM.
       + esplits; try eassumption. apply String.eqb_refl.
       + i. rewrite Heq in H2. ss.
   Qed.
-  
+
   Lemma isim_sget_tgt r g ps pt {Rs Rt} RR k st_src st_tgt i_src k_tgt :
     @isim r g Rs Rt RR ps true (st_src, i_src) (st_tgt, k_tgt (or_else (alist_find k st_tgt) tt↑))
     ⊢ @isim r g Rs Rt RR ps pt (st_src, i_src) (st_tgt, trigger (SGet k) >>= k_tgt).
@@ -399,7 +399,7 @@ Section SIM.
       + esplits; try eassumption. apply String.eqb_refl.
       + i. rewrite Heq in H2. ss.
   Qed.
-  
+
   Lemma isim_assume_src r g ps pt {Rs Rt} RR iP st_src st_tgt k_src i_tgt :
     (iP -∗ (@isim r g Rs Rt RR true pt (st_src, k_src tt) (st_tgt, i_tgt)))
     ⊢ @isim r g Rs Rt RR ps pt (st_src, trigger (Assume iP) >>= k_src) (st_tgt, i_tgt).
@@ -423,7 +423,7 @@ Section SIM.
     iIntros "X". iMod (Hx' with "X") as "[P X]". iPoseProof (Hx with "X P") as "SIM".
     iApply "SIM"; eauto.
   Qed.
-  
+
   Lemma isim_assume_tgt r g ps pt {Rs Rt} RR iP st_src st_tgt i_src k_tgt :
     (iP ∗ (@isim r g Rs Rt RR ps true (st_src, i_src) (st_tgt, k_tgt tt)))
     ⊢ @isim r g Rs Rt RR ps pt (st_src, i_src) (st_tgt, trigger (Assume iP) >>= k_tgt).
@@ -473,7 +473,7 @@ Section SIM.
 
   Lemma isim_triggerUB_src r g {Rs Rt} RR ps pt X st_src st_tgt (k_src : X -> _) i_tgt :
     ⊢ @isim r g Rs Rt RR ps pt (st_src, triggerUB >>= k_src) (st_tgt, i_tgt).
-  Proof using. 
+  Proof using.
     unfold triggerUB. ired. iApply isim_take_src.
     iIntros (x). destruct x.
   Qed.
@@ -596,7 +596,7 @@ Section SIM.
       (FIND : alist_find (Some fn) fl_tgt = Some f) :
     @isim r g Rs Rt RR ps true (st_src, i_src) (st_tgt, f varg >>= (λ ret, tau;; Ret ret) >>= k_tgt)
     ⊢ @isim r g Rs Rt RR ps pt (st_src, i_src) (st_tgt, trigger (Call fn varg) >>= k_tgt).
-  Proof using. 
+  Proof using.
     split; intros x wfx SIM; guclo msimC_spec; econs; esplits; eauto; econs; eauto.
   Qed.
 
@@ -611,7 +611,7 @@ Section SIM.
     des_ifs; ss.
     iApply isim_inline_tgt; eauto.
   Qed.
-  
+
   Lemma isim_spawn r g ps pt {Rs Rt} RR st_src st_tgt k_src k_tgt fn arg :
     (∀ tid, @isim r g Rs Rt RR true true (st_src, k_src tid) (st_tgt, k_tgt tid)) ⊢
     isim r g RR ps pt
@@ -639,7 +639,7 @@ Section SIM.
     { specialize (H eq_refl). inv H. }
     iApply isim_spawn. iFrame.
   Qed.
-  
+
   Lemma isim_yield r g ps pt {Rs Rt} RR st_src st_tgt k_src k_tgt tid :
     Ist st_src st_tgt ∗
     (∀ st_src0 st_tgt0,
@@ -687,7 +687,7 @@ Section SIM.
     - iApply isim_call_none; eauto.
     - unfold triggerUB. grind. iApply isim_take_src. iIntros (?). ss.
   Qed.
-  
+
   Lemma isim_spawn_none
     r g ps pt {Rs Rt} RR st_src st_tgt k_src i_tgt fn varg
     (CLOSED: contextual = closed)
@@ -711,7 +711,7 @@ Section SIM.
     - iApply isim_spawn_none; eauto.
     - unfold triggerUB. grind. iApply isim_take_src. iIntros (?). ss.
   Qed.
-  
+
   Lemma isim_call_mask_sandbox
     r g ps pt {Rs Rt} RR st_src st_tgt k_src i_tgt fn varg img msk scp
     (FIND: msk (Some fn) = false)
@@ -731,7 +731,7 @@ Section SIM.
     - rewrite SBRed.spawn H. iApply isim_triggerUB_src.
     - rewrite SBRed.spawn H. rewrite andb_false_r. iApply isim_triggerUB_src.
   Qed.
-  
+
   Lemma isim_progress r g {Rs Rt} RR st_src st_tgt i_src i_tgt :
     @isim g g Rs Rt RR false false (st_src, i_src) (st_tgt, i_tgt)
     ⊢ @isim r g Rs Rt RR true true (st_src, i_src) (st_tgt, i_tgt).
@@ -758,9 +758,9 @@ Section SIM.
     @isim r g Rs Rt RR false false sti_src sti_tgt
     ⊢ @isim r g Rs Rt RR ps pt sti_src sti_tgt.
   Proof using.
-    split; intros x wfx SIM. eapply msim_flag_down. eauto. 
+    split; intros x wfx SIM. eapply msim_flag_down. eauto.
   Qed.
-  
+
   Lemma isim_coind (r g : rel) A (P: A → _) RsA RtA RRA psA ptA srcA tgtA
     (COIND: ∀ (g0 : rel)
         (INC: ∀ Rs Rt RR ps pt src tgt, g Rs Rt RR ps pt src tgt ⊢ g0 Rs Rt RR ps pt src tgt)
@@ -797,7 +797,7 @@ Section SIM.
       }
     }
     { ii; eauto. }
-    { ii. inv PR. 
+    { ii. inv PR.
       uPred.unseal_once_in REL. destruct REL as [REL]. hexploit REL; eauto.
       { rewrite own.Own_eq /own.Own_def; uPred.unseal; rr.
         exists ε; rewrite right_id; ss. }
@@ -925,7 +925,7 @@ Section FancyReal.
 End FancyReal.
 
 Section FSEM.
-  Context `{_crisG: !crisG Γ Σ α β τ _S _I}.  
+  Context `{_crisG: !crisG Γ Σ α β τ _S _I}.
 
   Definition isim_fsem fl_src fl_tgt Ist contextual IstS IstE : relation (Any.t -> itree crisE Any.t) :=
   λ itr_src itr_tgt,
@@ -937,7 +937,7 @@ End FSEM.
 
 Module ISim. Section ISim.
   Import Mod.
-  Context `{!crisG Γ Σ α β τ _S _I}.  
+  Context `{!crisG Γ Σ α β τ _S _I}.
 
   Variable contextual: contextuality.
   Variable (ms_src ms_tgt : Mod.t).
